lib/MinMax.dfy
@@ -1,0 +1,33 @@
+module MinMax {
+
+  function method Min(a: int, b: int): int {
+    if a <= b then a else b
+  }
+
+  function method Max(a: int, b: int): int {
+    if a >= b then a else b
+  }
+
+  lemma MinProps(a: int, b: int)
+    ensures Min(a, b) <= a
+    ensures Min(a, b) <= b
+    ensures Min(a, b) == a || Min(a, b) == b
+    // ensures forall x :: x <= a && x <= b ==> x <= Min(a, b)
+  {
+  }
+
+  lemma MaxProps(a: int, b: int)
+    ensures a <= Max(a, b)
+    ensures b <= Max(a, b)
+    ensures Max(a, b) == a || Max(a, b) == b
+    // ensures forall x :: a <= x && b <= x ==> Max(a, b) <= x
+  {
+  }
+
+  lemma MinEqMax(a: int, b: int)
+    requires Min(a, b) == Max(a, b)
+    ensures a == b
+  {
+  }
+  
+}
