lib/SeqMethods.dfy
@@ -1,0 +1,142 @@
+include "Seq.dfy"
+
+module SeqMethods {
+  import opened Seq
+
+  method ReverseIter<T>(xs: seq<T>) returns (rev: seq<T>)
+    ensures rev == Reverse(xs)
+  {
+    rev := [];
+    var i := |xs|;
+    while i > 0
+      invariant i >= 0
+      invariant rev == Reverse(xs[i..])
+    {
+      i := i - 1;
+      rev := rev + [xs[i]];
+    }
+  }
+
+  method ReverseArray<T>(a: array<T>) returns (rev: array<T>)
+    ensures rev[..] == Reverse(a[..])
+  {
+    rev := new T[a.Length](i requires 0 <= i < a.Length reads a => a[a.Length - i - 1]);
+    ReverseIndexAll(a[..]);
+  }
+
+  method ReverseArrayInPlace<T>(a: array<T>) returns (rev: array<T>)
+    modifies a
+    ensures rev == a
+    ensures rev[..] == Reverse(old(a[..]))
+  {
+    var i := 0;
+    var j := a.Length - 1;
+    while i < j
+      invariant 0 <= i <= a.Length
+      invariant j < a.Length
+      invariant j == a.Length - i - 1
+      invariant forall k :: 0 <= k < i ==> a[k] == old(a[a.Length - k - 1])
+      invariant forall k :: j < k < a.Length ==> a[k] == old(a[a.Length - k - 1])
+      invariant forall k :: 0 <= i <= k <= j ==> a[k] == old(a[k])
+    {
+      a[i], a[j] := a[j], a[i];
+      i := i + 1;
+      j := j - 1;
+    }
+    ReverseIndexAll(old(a[..]));
+    return a;
+  }
+
+  method FoldlIter<A, B>(f: (A, B) -> A, z: A, xs: seq<B>) returns (r: A) 
+    ensures r == Foldl(f, z, xs)
+  {
+    r := z;
+    var i := 0;
+    while i < |xs|
+      invariant i <= |xs|
+      invariant r == Foldl(f, z, xs[..i])
+    {
+      r := f(r, xs[i]);
+      i := i + 1;
+      assert xs[..i] == xs[..i - 1] + [xs[i - 1]];
+    }
+    assert xs[..i] == xs;
+  }
+
+  method SumIter(xs: seq<int>) returns (s: int)
+    ensures s == Sum(xs)
+  {
+    var i := 0;
+    s := 0;
+    while i < |xs|
+      invariant i <= |xs|
+      invariant s == Sum(xs[..i])
+    {
+      s := s + xs[i];
+      i := i + 1;
+      assert xs[..i] == xs[..i - 1] + [xs[i - 1]];
+    }
+    assert xs[..i] == xs;
+  }
+
+  method CheckDistinct<T(==)>(xs: seq<T>) returns (r: bool)
+    ensures r <==> Distinct(xs)
+  {
+    var i := 0;
+    var s: set<T> := {};
+    while i < |xs|
+      invariant i <= |xs|
+      invariant forall x :: x in xs[..i] <==> x in s
+      invariant Distinct(xs[..i])
+    {
+      if xs[i] in s {
+        return false;
+      }
+      s := s + {xs[i]};
+      i := i + 1;
+    }
+    return true;
+  }
+
+  method CheckDistinctSubseq<T(==)>(xs: seq<T>, start: int, end: int) returns (r: bool)
+    requires 0 <= start <= end <= |xs|
+    ensures r <==> Distinct(xs[start..end])
+  {
+    var i := start;
+    var s: set<T> := {};
+    while i < end
+      invariant start <= i <= end
+      invariant forall x :: x in xs[start..i] <==> x in s
+      invariant Distinct(xs[start..i])
+    {
+      if xs[i] in s {
+        return false;
+      }
+      s := s + {xs[i]};
+      i := i + 1;
+      assert xs[start..i] == xs[start..i - 1] + [xs[i - 1]];
+    }
+    return true;
+  }
+
+  method CheckDistinctSubarray<T(==)>(a: array<T>, start: int, end: int) returns (r: bool)
+    requires 0 <= start <= end <= a.Length
+    ensures r <==> Distinct(a[start..end])
+  {
+    var i := start;
+    var s: set<T> := {};
+    while i < end
+      invariant start <= i <= end
+      invariant forall x :: x in a[start..i] <==> x in s
+      invariant Distinct(a[start..i])
+    {
+      if a[i] in s {
+        return false;
+      }
+      s := s + {a[i]};
+      i := i + 1;
+    }
+    return true;
+  }
+
+}
